{
 "cells": [
  {
   "cell_type": "markdown",
   "metadata": {},
   "source": [
    "Name: Ramas, Ron Patrick G. - 23102078 \\\n",
    "Discrete Math - CIS 1203 \\\n",
    "Group 2 - TTH 12:00 - 1:30 PM\n",
    "\n",
    "# **Assignment in Discrete Mathematics 2**\n",
    "\n",
    "---\n",
    "\n",
    "## **Lecture 1**\n",
    "\n",
    "1. Recall the definitions of a rational number, denoted as ${Q}$. Prove that the Euler's number ${e} = \\sum_{k=0}^\\infty \\frac{1}{k!} \\notin {Q}$. A factorial is defined as $\\\\k! = (k)(k-1)(k-2)(k-3)...,\\forall k \\in \\mathbb{Z}^+$, note that $0! = 1$. Furthermore, sum notation $\\sum_{k=0}^\\infty k=0+1+2+3+...+...$\n",
    "\n",
    "\tProof:\n",
    "\n",
    "\tSuppose $e$ is rational, such that $e=\\frac{n}{d}$, where $n$ and $d$ are positive integer.\n",
    "\n",
    "\t$\n",
    "\t\\begin{equation}\n",
    "\t\t\\frac{n}{d}=e\\sum_{k=0}^\\infty \\frac{1}{k!}\n",
    "\t\\end{equation}\n",
    "\t$\n",
    "\n",
    "\tBy multiplying both sides by $d!$, we get the following equation: \n",
    "\n",
    "\t$\n",
    "\t\\begin{align}\n",
    "\t\t\\frac{n}{d}d! & =d!\\sum_{k=0}^\\infty \\frac{1}{k!}\\\\\n",
    "\t\tn(d-1)! & = d! [\\frac{1}{0!}+\\frac{1}{1!}+\\frac{1}{2!}+...+\\frac{1}{d!}+\\frac{1}{(d+1)!}+\\frac{1}{(d+2)!}+\\frac{1}{(d+3)!}+...]\\\\\n",
    "\t\t&=(\\frac{d!}{0!}+\\frac{d!}{1!}+\\frac{d!}{2!}+...+\\frac{d!}{d!})+[\\frac{d!}{(d+1)!}+\\frac{d!}{(d+2)!}+\\frac{d!}{(d+3)!}+...]\\\\\n",
    "\t\t&=\\sum_{k=0}^d \\frac{d!}{k!}+\\sum_{k=d+1}^\\infty \\frac{d!}{k!} \n",
    "\t\\end{align}\n",
    "\t$\n",
    "\n",
    "\tThe term $n(d-1)!$ is clearly an integer. The first sum is also an integer, since $k \\leq d$. The second sum we can simplify as follows:\n",
    "\n",
    "\t$\n",
    "\t\\begin{equation}\n",
    "\t\t\\frac{1}{d+1}+\\frac{1}{(d+1)(d+2)}+\\frac{1}{(d+1)(d+2)(d+3)}+...\n",
    "\t\\end{equation}\n",
    "\t$\n",
    "\n",
    "\tThe second sum is clearly greater than **$0$**, and and we can see (by considering respective terms) that:\n",
    "\n",
    "\t$\n",
    "\t\\begin{equation}\n",
    "\t\t[\\frac{1}{d+1}+\\frac{1}{(d+1)(d+2)}+\\frac{1}{(d+1)(d+2)(d+3)}+...] < \\sum_{k=0}^\\infty (\\frac{1}{d+1})^{(k+1)}\n",
    "\t\\end{equation}\n",
    "\t$\n",
    "\n",
    "\tThe right-hand side of the inequality is a geometric series, and we used the formula to show that the second sum is going to be less than **$1$**\n",
    "\n",
    "\t$\n",
    "\t\\begin{align}\n",
    "\t\t\\sum_{k=0}^\\infty (\\frac{1}{d+1})^{(k+1)} & =[\\frac{1}{d+1}+\\frac{1}{(d+1)^2}+\\frac{1}{(d+1)^3}+...]\\\\\n",
    "\t\t& =\\frac{\\frac{1}{d+1}}{1-\\frac{1}{d+1}}=\\frac{1}{d} \\leq 1\n",
    "\t\\end{align}\n",
    "\t$\n",
    "\n",
    "\tWith this logical statement, the second sum is greater than **$0$** and less than **$1$**, which is not an integer. This is a contradiction, since $n(d-1)!$ is an integer, and the second sum is not an integer.\n",
    "\n",
    "\t$\n",
    "\t\\begin{equation}\n",
    "\t\tn(d-1)! \\neq \\sum_{k=0}^d \\frac{d!}{k!}+\\sum_{k=d+1}^\\infty \\frac{d!}{k!}\n",
    "\t\\end{equation}\n",
    "\t$\n",
    "\n",
    "\tTherefore, $e$ is irrational since $\\mathbb{Z}=\\overline{\\mathbb{Z}}$ is simply impossible.\n",
    "\n",
    "---\n",
    "\n",
    "2. Prove Minkowski's Inequality for sums, $\\forall p>1,(a_k, b_k)>0$:\n",
    "\n",
    "\t$\n",
    "\t\\begin{equation}\n",
    "\t\t(\\sum_{k=1}^n(|a_k|+|b_k|)^p)^{\\frac{1}{p}} \\leq (\\sum_{k=1}^n |a_k|^p)^{\\frac{1}{p}}+(\\sum_{k=1}^n |b_k|^p)^{\\frac{1}{p}}\n",
    "\t\\end{equation}\n",
    "\t$\n",
    "\n",
    "\tProof:\n",
    "\n",
    "\t$\n",
    "\t\\begin{equation}\n",
    "\t\t(\\sum_{k=1}^n |a_k+b_k|^p)^{\\frac{1}{p}} \\leq (\\sum_{k=1}^n |a_k|^p)^{\\frac{1}{p}}+(\\sum_{k=1}^n |b_k|^p)^{\\frac{1}{p}}\n",
    "\t\\end{equation}\n",
    "\t$\n",
    "\n",
    "\tTo prove Minkowski's inequality, we can use Hölder's inequality:\n",
    "\n",
    "\tIf $p>1$ and $q>1$ are such that\n",
    "\n",
    "\t$\n",
    "\t\\begin{equation}\n",
    "\t\t\\frac{1}{p}+\\frac{1}{q}=1\n",
    "\t\\end{equation}\n",
    "\t$\n",
    "\n",
    "\tthen for all $x$ and $y \\in \\R^n$ we have\n",
    "\n",
    "\t$\n",
    "\t\\begin{equation}\n",
    "\t\t\\sum_{k=1}^n |x_ky_k| \\leq (\\sum_{k=1}^n |x_k|^p)^{\\frac{1}{p}} (\\sum_{k=1}^n |y_k|^q)^{\\frac{1}{q}}\n",
    "\t\\end{equation}\n",
    "\t$\n",
    "\n",
    "\tProof of Minkowski's Inequality. Observe that $(\\sum_{k=1}^n(|a_k|+|b_k|)^p)^{\\frac{1}{p}} \\leq (\\sum_{k=1}^n |a_k|^p)^{\\frac{1}{p}}+(\\sum_{k=1}^n |b_k|^p)^{\\frac{1}{p}}$ holds for the case $p=1$ by summing both sides of the simple triangle inequality.\n",
    "\n",
    "\t$\n",
    "\t\\begin{equation}\n",
    "\t\t|a_k+b_k| \\leq |a_k|+|b_k|\n",
    "\t\\end{equation}\n",
    "\t$\n",
    "\n",
    "\tWe now concentrate on the case $p>1$. For this case we show:\n",
    "\n",
    "\t$\n",
    "\t\\begin{equation}\n",
    "\t\t(\\sum_{k=1}^n(|a_k|+|b_k|)^p)^{\\frac{1}{p}} \\leq (\\sum_{k=1}^n |a_k|^p)^{\\frac{1}{p}}+(\\sum_{k=1}^n |b_k|^p)^{\\frac{1}{p}}\n",
    "\t\\end{equation}\n",
    "\t$\n",
    "\n",
    "\tso that the simple triangle inequality will imply $(\\sum_{k=1}^n(|a_k|+|b_k|)^p)^{\\frac{1}{p}} \\leq (\\sum_{k=1}^n |a_k|^p)^{\\frac{1}{p}}+(\\sum_{k=1}^n |b_k|^p)^{\\frac{1}{p}}$. For all $a_k$ and $b_k$, we have:\n",
    "\n",
    "\t$\n",
    "\t\\begin{align}\n",
    "\t\t(|a_k|+|b_k|)^p & =(|a_k|+|b_k|)(|a_k|+|b_k|)^{p-1}\\\\\n",
    "\t\t& =|a_k|(|a_k|+|b_k|)^{p-1}+|b_k|(|a_k|+|b_k|)^{p-1}\n",
    "\t\\end{align}\n",
    "\t$\n",
    "\n",
    "\tSumming both sides of this, we obtain:\n",
    "\n",
    "\t$\n",
    "\t\\begin{equation}\n",
    "\t\t(\\sum_{k=1}^n (|a_k|+|b_k|)^p)^{\\frac{1}{p}} \\leq (\\sum_{k=1}^n |a_k|^p)^{\\frac{1}{p}}+(\\sum_{k=1}^n |b_k|^p)^{\\frac{1}{p}}\n",
    "\t\\end{equation}\n",
    "\t$\n",
    "\n",
    "\tNow, applying Hölder's inequality to both terms to the right of the equation, we get:\n",
    "\n",
    "\t$\n",
    "\t\\begin{equation}\n",
    "\t\t\\sum_{k=1}^n |a_k|(|a_k|+|b_k|)^{p-1} \\leq (\\sum_{k=1}^n |a_k|^p)^{\\frac{1}{p}}(\\sum_{k=1}^n[(|a_k|+|b_k|)^{p-1}]^q)^{\\frac{1}{q}}\n",
    "\t\\end{equation}\n",
    "\t$\n",
    "\n",
    "\t$\n",
    "\t\\begin{equation}\n",
    "\t\t\\sum_{k=1}^n |b_k|(|a_k|+|b_k|)^{p-1} \\leq (\\sum_{k=1}^n |b_k|^p)^{\\frac{1}{p}}(\\sum_{k=1}^n[(|a_k|+|b_k|)^{p-1}]^q)^{\\frac{1}{q}}\n",
    "\t\\end{equation}\n",
    "\t$\n",
    "\n",
    "\tCombining $(\\sum_{k=1}^n (|a_k|+|b_k|)^p)^{\\frac{1}{p}} \\leq (\\sum_{k=1}^n |a_k|^p)^{\\frac{1}{p}}+(\\sum_{k=1}^n |b_k|^p)^{\\frac{1}{p}}$ with the previous two equations, we obtain:\n",
    "\n",
    "\t$\n",
    "\t\\begin{align}\n",
    "\t\t\\sum_{k=1}^n (|a_k|+|b_k|)^p & \\leq [(\\sum_{k=1}^n |a_k|^p)^{\\frac{1}{p}}+(\\sum_{k=1}^n |b_k|^p)^{\\frac{1}{p}}] (\\sum_{k=1}^n(|a_k|+|b_k|)^{(p-1)q})^{\\frac{1}{q}}\\\\\n",
    "\t\t& =[(\\sum_{k=1}^n |a_k|^p)^{\\frac{1}{p}}+(\\sum_{k=1}^n |b_k|^p)^{\\frac{1}{p}}] (\\sum_{k=1}^n(|a_k|+|b_k|^p))^{\\frac{1}{q}}\n",
    "\t\\end{align}\n",
    "\t$\n",
    "\n",
    "\twhere we have used $\\frac{1}{p}+\\frac{1}{q}=1$, rearranging the previous equation, we have:\n",
    "\n",
    "\t$\n",
    "\t\\begin{equation}\n",
    "\t\t\\frac{\\sum_{k=1}^n (|a_k|+|b_k|)^p}{(\\sum_{k=1}^n (|a_k|+|b_k|)^p)^{\\frac{1}{q}}} \\leq (\\sum_{k=1}^n |a_k|^p)^{\\frac{1}{p}}+(\\sum_{k=1}^n |b_k|^p)^{\\frac{1}{p}}\n",
    "\t\\end{equation}\n",
    "\t$\n",
    "\n",
    "---\n",
    "\n",
    "3. Prove the triangle triangle inequality $|x+y| \\leq |x|+|y|,\\forall (x,y) \\in \\R$:\n",
    "\n",
    "\tCase 1: Both x and y are nonnegative:\n",
    "\n",
    "\t- If $x \\geq 0$ and $y \\geq 0$, then $|x + y| = x + y$ and $|x| + |y| = x + y$. Since $x + y \\leq x + y$, the inequality holds.\n",
    "\n",
    "\tCase 2: Both $x$ and $y$ are nonpositive:\n",
    "\n",
    "\t- If $x \\leq 0$ and $y \\leq 0$, then $|x + y| = −(x + y)$ and $|x| + |y| = (−x) + (−y)$. Since $−(x + y) \\leq (−x) + (−y)$,\n",
    "\tthe inequality holds.\n",
    "\n",
    "\tCase 3: One of x or y is nonnegative and the other is nonpositive:\n",
    "\n",
    "\t- If $x \\geq 0$ and $y \\leq 0$, then $|x + y| = |x − (−y)|$ and $|x| + |y| = x + (−y)$. Since $|x − (−y)| \\leq x + (−y)$,\n",
    "\tthe inequality holds.\n",
    "\t- This method also applies to $x \\leq 0$ and $y \\geq 0$.\n",
    "\n",
    "\tBy examining all possible cases, we have shown that the triangle inequality holds $\\forall(x, y) \\in \\R$. Therefore,the inequality\n",
    "\t$|x + y| \\leq |x| + |y|$ is proven.\n",
    "\n",
    "---\n",
    "\n",
    "4. Prove Sedrakayan's Lemma $\\forall u_i,v_i \\in \\R^+$:\n",
    "\n",
    "\t$\n",
    "\t\\begin{equation}\n",
    "\t\t\\frac{(\\sum_{i=1}^n u_i)^2}{\\sum_{i=1}^n v_i} \\leq \\sum_{i=1}^n \\frac{(u_i)^2}{v_i}\n",
    "\t\\end{equation}\n",
    "\t$\n",
    "\n",
    "\tTo prove the Sedrakayan's Lemma, we use Cauchy-Schwarz Inequality.\n",
    "\n",
    "\tLet's denote $x_i=\\sqrt{v_i}$ and $y_i=u_i$. Then the given inequality becomes:\n",
    "\n",
    "\t$\n",
    "\t\\begin{equation}\n",
    "\t\t(\\frac{\\sum_{i=1}^n x_iy_i}{\\sqrt{\\sum_{i=1}^n v_i}})^2 \\leq \\sum_{i=1}^n \\frac{(x_i)^2(y_i)^2}{v_i}\n",
    "\t\\end{equation}\n",
    "\t$\n",
    "\n",
    "\tThis is essentially the squared form of the Cauchy-Schwarz Inequality, which states\n",
    "\n",
    "\t$\n",
    "\t\\begin{equation}\n",
    "\t\t(\\sum_{i=1}^n a_ib_i)^2 \\leq (\\sum_{i=1}^n a_i^2)(\\sum_{i=1}^n b_i^2)\n",
    "\t\\end{equation}\n",
    "\t$\n",
    "\n",
    "\twhere\n",
    "\n",
    "\t$\n",
    "\t\\begin{equation}\n",
    "\t\ta_i=x_i \\sqrt{\\frac{v_i}{\\sum_{i=1}^n v_i}}\n",
    "\t\\end{equation}\n",
    "\t$\n",
    "\n",
    "\t$\n",
    "\t\\begin{equation}\n",
    "\t\tb_i=\\frac{y_i}{\\sqrt{\\frac{v_i}{\\sum_{i=1}^n v_i}}}\n",
    "\t\\end{equation}\n",
    "\t$\n",
    "\n",
    "\tBy applying the Cauchy-Schwarz Inequality to the previous two equations, we get:\n",
    "\n",
    "\t$\n",
    "\t\\begin{equation}\n",
    "\t\t(\\sum_{i=1}^n x_iy_i \\sqrt{\\frac{v_i}{\\sum_{i=1}^n v_i}})^2 \\leq (\\sum_{i=1}^n (x_i)^2 \\frac{v_i}{\\sum_{i=1}^n v_i})(\\sum_{i=1}^n (y_i)^2 \\frac{1}{\\frac{v_i}{\\sum_{i=1}^n v_i}})\n",
    "\t\\end{equation}\n",
    "\t$\n",
    "\n",
    "\tSimplify:\n",
    "\n",
    "\t$\n",
    "\t\\begin{equation}\n",
    "\t\t(\\sum_{i=1}^n x_iy_i)^2 \\leq (\\sum_{i=1}^n (x_i)^2)(\\sum_{i=1}^n (y_i)^2)\n",
    "\t\\end{equation}\n",
    "\t$\n",
    "\n",
    "\tWhich is equivalent to:\n",
    "\n",
    "\t$\n",
    "\t\\begin{equation}\n",
    "\t\t(\\frac{\\sum_{i=1}^n u_i}{\\sqrt{\\sum_{i=1}^n v_i}})^2 \\leq \\sum_{i=1}^n \\frac{(u_i)^2}{v_i}\n",
    "\t\\end{equation}\n",
    "\t$\n",
    "\n",
    "\tHence, Sedrakayan's Lemma is proved.\n",
    "\n",
    "---\n",
    "\n",
    "5. Consider the functions $f(x)=2x+1$, $g(x)=2y-1$, $j(x)=|f(x)+g(x)|$, and $h(x)=j(x)^2$, show for the following inequality that:\n",
    "\n",
    "\t$\n",
    "\t\\begin{equation}\n",
    "\t\t\\sqrt{|f(x)|^2} \\geq \\sqrt{h(x)}-\\sqrt{|g(x)|^2},\\forall(x,y)\\in \\mathbb{Z}^+\n",
    "\t\\end{equation}\n",
    "\t$\n",
    "\n",
    "\tWith the given functions, we can substitute $f(x)$ and $g(x)$ into $j(x)$:\n",
    "\n",
    "\t$\n",
    "\t\\begin{equation}\n",
    "\t\tj(x)=|(2x+1)+(2y-1)| = |2x+2y| = 2|x+y|\n",
    "\t\\end{equation}\n",
    "\t$\n",
    "\n",
    "\tWith this, we can also find $h(x)$:\n",
    "\n",
    "\t$\n",
    "\t\\begin{equation}\n",
    "\t\th(x)=j(x)^2=(2|x+y|)^2=4(x+y)^2\n",
    "\t\\end{equation}\n",
    "\t$\n",
    "\n",
    "\tWe can simplify the inequalities:\n",
    "\n",
    "\t$\n",
    "\t\\begin{equation}\n",
    "\t\t\\sqrt{h(x)}=\\sqrt{4(x+y)^2}=2|x+y|\n",
    "\t\\end{equation}\n",
    "\t$\n",
    "\n",
    "\t$\n",
    "\t\\begin{equation}\n",
    "\t\t\\sqrt{|f(x)|^2}=\\sqrt{(2x+y)^2}=|2x+1|\n",
    "\t\\end{equation}\n",
    "\t$\n",
    "\n",
    "\t$\n",
    "\t\\begin{equation}\n",
    "\t\t\\sqrt{|g(x)|^2}=\\sqrt{(2y+1)^2}=|2y+1|\n",
    "\t\\end{equation}\n",
    "\t$\n",
    "\n",
    "\tNow we get:\n",
    "\n",
    "\t$\n",
    "\t\\begin{equation}\n",
    "\t\t|2x+1| \\geq 2|x+y| - |2y-1|\n",
    "\t\\end{equation}\n",
    "\t$\n",
    "\n",
    "\tWhen analyzing the different absolute values in the equation as well as from the given, we can see that:\n",
    "\n",
    "\t- For $(2x+1)$, it's always positive for $(x\\in \\mathbb{Z}^+)$, hence $(|2x+1| =2x+1)\n",
    "\t- For $(2y-1)$, if $(y \\geq 1)$, then $(|2y-1| = 2y-1)\n",
    "\t- For $(x+y)$, since $(x,y) \\in \\mathbb{Z}^+$, then $|x+y| = (x+y)$\n",
    "\n",
    "\tTherefore, the equality can be simplified down to:\n",
    "\n",
    "\t$\n",
    "\t\\begin{equation}\n",
    "\t\t2x+1 \\geq 2(x+y)-(2y-1)\n",
    "\t\\end{equation}\n",
    "\t$\n",
    "\n",
    "\t$\n",
    "\t\\begin{equation}\n",
    "\t\t2x+1 \\geq 2x+2y-2y+1\n",
    "\t\\end{equation}\n",
    "\t$\n",
    "\n",
    "\t$\n",
    "\t\\begin{equation}\n",
    "\t\t2x+1 \\geq 2x+1\n",
    "\t\\end{equation}\n",
    "\t$\n",
    "\n",
    "\tTherefore, the original inequality is proven since $2x+1 \\geq 2x+1$ is always true regardless of the value of $x$/\n",
    "\n",
    "---\n",
    "\n",
    "6. Prove Sedrakayan's Lemma if $u_i, v_i$ are square roots of an even integer:\n",
    "\n",
    "\t$\n",
    "\t\\begin{equation}\n",
    "\t\t\\frac{(\\sum_{i=1}^n u_i)^2}{\\sum_{i=1}^n v_i} \\leq \\sum_{i=1}^n \\frac{(u_i)^2}{v_i}\n",
    "\t\\end{equation}\n",
    "\t$\n",
    "\n",
    "\tSince $u$ and $v$ are square roots of even integers, we can replace them with $\\sqrt{2a_i}$ and $\\sqrt{2b_i}$ respectively.\n",
    "\n",
    "\tWith this, we can replace the left-hand side of the equation with:\n",
    "\n",
    "\t$\n",
    "\t\\begin{equation}\n",
    "\t\t\\frac{(\\sum_{i=1}^n u_i)^2}{\\sum_{i=1}^n v_i}=\\frac{(\\sum_{i=1}^n \\sqrt{2a_i})^2}{\\sum_{i=1}^n \\sqrt{2b_i}}\n",
    "\t\\end{equation}\n",
    "\t$\n",
    "\n",
    "\tSimplifying the numerator and the denominator:\n",
    "\n",
    "\t$\n",
    "\t\\begin{equation}\n",
    "\t\t\\frac{(\\sum_{i=1}^n \\sqrt{2a_i})^2}{\\sum_{i=1}^n \\sqrt{2b_i}}=\\frac{2(\\sum_{i=1}^n \\sqrt{a_i})^2}{2\\sum_{i=1}^n \\sqrt{b_i}}=\\frac{(\\sum_{i=1}^n \\sqrt{2a_i})^2}{\\sum_{i=1}^n \\sqrt{2b_i}}\n",
    "\t\\end{equation}\n",
    "\t$\n",
    "\n",
    "\tNow, let's compute the right-hand side:\n",
    "\n",
    "\t$\n",
    "\t\\begin{equation}\n",
    "\t\t\\sum_{i=1}^n\\frac{u_i^2}{v_i}=\\sum_{i=1}^n\\frac{(\\sqrt{2a_i}^2)}{\\sqrt{2b_i}}=\\sum_{i=1}^n\\frac{2a_i}{\\sqrt{2b_i}}=\\sum_{i=1}^n\\frac{2a_i}{\\sqrt{2}\\sqrt{b_i}}=\\sum_{i=1}^n\\frac{2a_i}{\\sqrt{2b_i}}=\\sqrt{2}\\sum_{i=1}^n\\frac{a_i}{\\sqrt{b_i}}\n",
    "\t\\end{equation}\n",
    "\t$\n",
    "\n",
    "\tSo the inequality becomes:\n",
    "\n",
    "\t$\n",
    "\t\\begin{equation}\n",
    "\t\t\\frac{(\\sum_{i=1}^n\\sqrt{a_i})^2}{\\sum_{i=1}^n\\sqrt{b_i}}\\leq\\sqrt{2}\\sum_{i=1}^n\\frac{a_i}{\\sqrt{b_i}}\n",
    "\t\\end{equation}\n",
    "\t$\n",
    "\n",
    "\tWe can now analyze and prove this inequality utilizing the Cauchy-Schwarz inequality.\n",
    "\n",
    "\tBy the Cauchy-Schwarz inequality applied to the sequences $(\\sqrt{a_i})$ and $(\\frac{1}{\\sqrt{b_i}})$:\n",
    "\n",
    "\t$\n",
    "\t\\begin{equation}\n",
    "\t\t(\\sum_{i=1}^n\\sqrt{a_i}\\cdot\\frac{1}{\\sqrt{b_i}})^2\\leq(\\sum_{i=1}^n\\sqrt{(a_i)^2})(\\sum_{i=1}^n(\\frac{1}{\\sqrt{b_i}})^2)\n",
    "\t\\end{equation}\n",
    "\t$\n",
    "\n",
    "\tSimplify the term:\n",
    "\n",
    "\t$\n",
    "\t\\begin{equation}\n",
    "\t\t(\\sum_{i=1}^n\\frac{\\sqrt{a_i}}{\\sqrt{b_i}})^2\\leq(\\sum_{i=1}^n a_i)(\\sum_{i=1}^n\\frac{1}{b_i})\n",
    "\t\\end{equation}\n",
    "\t$\n",
    "\n",
    "\tTo apply this to our problem, we can rewrite the original left-hand side as follows:\n",
    "\n",
    "\t$\n",
    "\t\\begin{equation}\n",
    "\t\t\\frac{(\\sum_{i=1}^n\\sqrt{a_i})^n}{\\sum_{i=1}^n\\sqrt{b_i}}=\\frac{(\\sum_{i=1}^n\\sqrt{a_i}\\cdot\\sqrt{b_i}\\cdot\\frac{1}{\\sqrt{b_i}})^2}{\\sum_{i=1}^n\\sqrt{b_i}}\n",
    "\t\\end{equation}\n",
    "\t$\n",
    "\n",
    "\tUsing the Cauchy-Schwarz inequality result:\n",
    "\n",
    "\t$\n",
    "\t\\begin{equation}\n",
    "\t\t(\\sum_{i=1}^n\\sqrt{a_i}\\cdot\\frac{1}{\\sqrt{b_i}})^2\\leq(\\sum_{i=1}^n a_i)(\\sum_{i=1}^n\\frac{1}{b_i})\n",
    "\t\\end{equation}\n",
    "\t$\n",
    "\n",
    "\tThus:\n",
    "\n",
    "\t$\n",
    "\t\\begin{equation}\n",
    "\t\t\\frac{(\\sum_{i=1}^n\\sqrt{a_i})^2}{\\sum_{i=1}^n\\sqrt{b_i}}\\leq\\frac{(\\sum_{i=1}^n a_i)}{\\sum_{i=1}^n\\frac{1}{b_i}}\n",
    "\t\\end{equation}\n",
    "\t$\n",
    "\n",
    "\tTherefore, we have shown:\n",
    "\n",
    "\t$\n",
    "\t\\begin{equation}\n",
    "\t\t\\frac{(\\sum_{i=1}^n u_i)^2}{\\sum_{i=1}^n v_i}\\leq\\sum_{i=1}^n\\frac{u_i^2}{v_i}\n",
    "\t\\end{equation}\n",
    "\t$"
   ]
  },
  {
   "cell_type": "markdown",
   "metadata": {},
   "source": []
  }
 ],
 "metadata": {
  "language_info": {
   "name": "python"
  }
 },
 "nbformat": 4,
 "nbformat_minor": 2
}
